Implementing tactic macro and adding some theorems to be proved

Coq/CSP/semantics_trace.v
@@ -104,11 +104,12 @@ Proof.
       + apply prefix_rule.
       + apply sos_empty_rule.
 Qed.
-
+*)
 Definition CH_CHOOSE := Channel {{"select", "keep", "return"}}.
 Definition P_CHOOSE := "CHOOSE" ::= "select" --> ("keep" --> SKIP
-                                                [] "return" --> "CHOOSE").
+                                                [] "return" --> ProcRef "CHOOSE").
 Definition S_CHOOSE := Spec [CH_CHOOSE] [P_CHOOSE].
+(*
 Example CHOOSE_trace1 : traceR S_CHOOSE "CHOOSE" ["select" ; "keep"].
 Proof.
   unfold traceR. simpl.
@@ -156,18 +157,18 @@ Proof.
         + apply prefix_rule.
       * apply sos_empty_rule.
 Qed.
-
+*)
 Definition CH_TEAM := Channel {{"lift_piano", "lift_table"}}.
-Definition PETE := "PETE" ::= "lift_piano" --> "PETE"
-                              |~| "lift_table" --> "PETE".
+Definition PETE := "PETE" ::= "lift_piano" --> ProcRef "PETE"
+                              |~| "lift_table" --> ProcRef "PETE".
 
-Definition DAVE := "DAVE" ::= "lift_piano" --> "DAVE"
-                              |~| "lift_table" --> "DAVE".
+Definition DAVE := "DAVE" ::= "lift_piano" --> ProcRef "DAVE"
+                              |~| "lift_table" --> ProcRef "DAVE".
 
-Definition TEAM := "TEAM" ::= "PETE" [| {{"lift_piano", "lift_table"}} |] "DAVE".
+Definition TEAM := "TEAM" ::= ProcRef "PETE" [| {{"lift_piano", "lift_table"}} |] ProcRef "DAVE".
 
 Definition S_TEAM := Spec [CH_TEAM] [PETE ; DAVE ; TEAM].
-
+(*
 Example TEAM_trace1 : traceR S_TEAM "TEAM" ["lift_piano"].
 Proof.
   unfold traceR. simpl.
@@ -512,32 +513,85 @@ Qed.
 Ltac solve_trace := unfold traceR; simpl;
   repeat (
     match goal with
+    (* Empty trace *)
     | |- traceR' _ _ nil => apply empty_trace_rule
-    | |- traceR' _ ?P _ =>  match P with
-                            | _ --> _ => eapply event_trace_rule
-                            | ProcRef _ => eapply tau_trace_rule
-                            end
-    | |- (_ # ?e --> _ // Event ?e ==> _) => apply prefix_rule
-    | |- (_ # ProcRef _ // Tau ==> _) => eapply reference_rule ; reflexivity
+    (* Non-empty trace *)
+    | |- traceR' _ ?P (?h :: _) =>
+      match P with
+      (* Prefix *)
+      | h --> _  => eapply event_trace_rule
+      (* Process unfolding *)
+      | ProcRef _ => eapply tau_trace_rule
+      (* External choice *)
+      | h --> _ [] _ => eapply event_trace_rule
+      | _ [] h --> _ => eapply event_trace_rule
+      | ProcRef _ [] _ => eapply tau_trace_rule
+      | _ [] ProcRef _ => eapply tau_trace_rule
+      (* Internal choice *)
+      | h --> ?Q |~| _ => apply tau_trace_rule with (P' := h --> Q)
+      | _ |~| h --> ?Q => apply tau_trace_rule with (P' := h --> Q)
+      | _ |~| _ => eapply tau_trace_rule
+      (* Interleaving *)
+      | h --> ?Q ||| ?Q' => apply event_trace_rule with (P' := ?Q ||| ?Q')
+      | ?Q ||| h --> ?Q' => apply event_trace_rule with (P' := ?Q ||| ?Q')
+      end
+    (* SOS Prefix rule *)
+    | |- (_ # (?e --> _) // Event ?e ==> _) => apply prefix_rule
+    (* SOS Reference rule *)
+    | |- (_ # (ProcRef _) // Tau ==> _) => eapply reference_rule
+    (* SOS External choice rule *)
+    | |- (_ # (?e --> _) [] _ // Event ?e ==> _) => eapply ext_choice_left_rule
+    | |- (_ # _ [] (?e --> _) // Event ?e ==> _) => eapply ext_choice_right_rule
+    (* SOS Internal choice *)
+    | |- (_ # ?P |~| ?Q // Tau ==> ?P) => eapply int_choice_left_rule
+    | |- (_ # ?P |~| ?Q // Tau ==> ?Q) => eapply int_choice_right_rule
+    (* SOS Interleaving *)
+    | |- (_ # ?e --> ?P ||| ?Q // Event ?e ==> ?P ||| ?Q) => eapply interleave_left_rule
+    | |- (_ # ?P ||| ?e --> ?Q // Event ?e ==> ?P ||| ?Q) => eapply interleave_right_rule
+    (* Prove not equal *)
+    | |- _ <> _ => unfold not; let H := fresh "H" in intros H; inversion H
+    (* Prove equal *)
+    | |- _ = _ => reflexivity
+    (* None of the above *)
+    | |- _ => fail
     end).
+
+Example CHOOSE_trace1 : traceR S_CHOOSE "CHOOSE" ["select" ; "return" ; "select" ; "keep"].
+Proof.
+  solve_trace.
+Qed.
 
 Example LIGHT_trace2 : traceR S_LIGHT "LIGHT" ["on"; "off" ; "on"].
 Proof.
   solve_trace.
 Qed.
 
-Theorem trace_eq :
-  forall (C : specification) (P : string) (exT : extendedTrace),
-    extendedTraceR C P exT <-> traceR C P (get_trace exT).
+Example TEAM_trace1 : traceR S_TEAM "PETE" ["lift_piano" ; "lift_table"].
 Proof.
-  intros. split.
-  - intros. destruct C, proc_list; try inversion H.
-    * induction P, exT; destruct p, name; try apply empty_trace_rule.
-      + induction proc_list.
-        { inversion H. }
-        (* TODO It seems that, no matter what I do, I can't get rid of the
-          extra element in the process list inside the specification so that
-          I can apply the induction hypothesis. *)
-        Abort.
+  solve_trace.
+Qed.
+
+Theorem extended_to_trace :
+  forall (C : specification) (P : string) (exT : extendedTrace),
+    extendedTraceR C P exT -> traceR C P (get_trace exT).
+Proof. Admitted.
+
+Theorem trace_to_extended :
+  forall (C : specification) (P : string) (t : trace),
+    traceR C P t ->
+    exists (exT : extendedTrace),
+      t = get_trace exT /\ extendedTraceR C P exT.
+Proof.
+  intros.
+  - destruct C. induction t.
+    * exists nil. split.
+      + reflexivity.
+      + destruct P, proc_list; try inversion H.
+        {
+          destruct p, name.
+          { 
+            unfold extendedTraceR; simpl. unfold extendedTraceR'.
+            exists body. apply sos_empty_rule.
+          } Admitted.
 
 Local Close Scope string.
